proof/correctness/.dir-locals.el
@@ -1,5 +1,5 @@
 ((easycrypt-mode .
   ((eval .
     (cl-flet ((pre (s) (concat (locate-dominating-file buffer-file-name ".dir-locals.el") s)))
-           (setq easycrypt-load-path `(,(pre ".") ,(pre "../spec"), 
+           (setq easycrypt-load-path `(,(pre ".") ,(pre "../spec"), (pre "../../sha3/proof/"),
              (pre "./extraction"),(pre "../security"), (pre "../eclib"), (pre "avx2/extraction"))))))))
